Progress in Coq model.

coq/Expr.v
@@ -4,13 +4,19 @@ Require Import Coq.Unicode.Utf8.
 From mathcomp Require Import ssreflect ssrfun ssrbool eqtype ssrnat choice ssrint
   rat ssralg ssrnum.
 
-From extructures Require Import ord.
+From extructures Require Import ord fset.
 
 From void Require Import void.
 
 From deriving Require Import deriving.
 
-Inductive var := Var of string & nat.
+Set Implicit Arguments.
+Unset Strict Implicit.
+Unset Printing Implicit Defensive.
+
+Local Open Scope fset_scope.
+
+Inductive var := Var {vname : string; vnum : nat}.
 
 Definition var_indMixin := Eval simpl in [indMixin for var_rect].
 Canonical var_indType := IndType _ var var_indMixin.
@@ -38,6 +44,7 @@ Inductive trunc_op :=
 | Ceil
 | Floor.
 
+Unset Elimination Schemes.
 Inductive bexpr :=
 | BConst of bool
 | BEqB   of bexpr & bexpr
@@ -61,51 +68,92 @@ with qexpr :=
 | QTest  of bexpr & qexpr & qexpr
 | QArith of arith_op & qexpr & qexpr
 | QOfZ   of zexpr.
+Set Elimination Schemes.
+
+Scheme bexpr_rect := Induction for bexpr Sort Type
+with   zexpr_rect := Induction for zexpr Sort Type
+with   qexpr_rect := Induction for qexpr Sort Type.
+
+Combined Scheme expr_rect from bexpr_rect, zexpr_rect, qexpr_rect.
+
+Scheme bexpr_ind := Induction for bexpr Sort Prop
+with   zexpr_ind := Induction for zexpr Sort Prop
+with   qexpr_ind := Induction for qexpr Sort Prop.
+
+Combined Scheme expr_ind from bexpr_ind, zexpr_ind, qexpr_ind.
 
 Section Eval.
 
 Implicit Types (be : bexpr) (ze : zexpr) (qe : qexpr).
 
-Variable f : var → int.
-
-Fixpoint eval_bexpr be : bool :=
+Fixpoint eval_bexpr f be : bool :=
   match be with
   | BConst b => b
-  | BEqB be1 be2 => eval_bexpr be1 == eval_bexpr be2
-  | BEqZ ze1 ze2 => eval_zexpr ze1 == eval_zexpr ze2
-  | BEqQ qe1 qe2 => eval_qexpr qe1 == eval_qexpr qe2
-  | BTest be be1 be2 => if eval_bexpr be then eval_bexpr be1
-                        else eval_bexpr be2
-  | BCompZ Leq ze1 ze2 => (eval_zexpr ze1 <= eval_zexpr ze2)%R
-  | BCompZ Ltq ze1 ze2 => (eval_zexpr ze1 <  eval_zexpr ze2)%R
-  | BCompQ Leq qe1 qe2 => (eval_qexpr qe1 <= eval_qexpr qe2)%R
-  | BCompQ Ltq qe1 qe2 => (eval_qexpr qe1 <  eval_qexpr qe2)%R
-  | BLogOp And be1 be2 => eval_bexpr be1 && eval_bexpr be2
-  | BLogOp Or  be1 be2 => eval_bexpr be1 || eval_bexpr be2
-  | BNot be => ~~ eval_bexpr be
+  | BEqB be1 be2 => eval_bexpr f be1 == eval_bexpr f be2
+  | BEqZ ze1 ze2 => eval_zexpr f ze1 == eval_zexpr f ze2
+  | BEqQ qe1 qe2 => eval_qexpr f qe1 == eval_qexpr f qe2
+  | BTest be be1 be2 => if eval_bexpr f be then eval_bexpr f be1
+                        else eval_bexpr f be2
+  | BCompZ Leq ze1 ze2 => (eval_zexpr f ze1 <= eval_zexpr f ze2)%R
+  | BCompZ Ltq ze1 ze2 => (eval_zexpr f ze1 <  eval_zexpr f ze2)%R
+  | BCompQ Leq qe1 qe2 => (eval_qexpr f qe1 <= eval_qexpr f qe2)%R
+  | BCompQ Ltq qe1 qe2 => (eval_qexpr f qe1 <  eval_qexpr f qe2)%R
+  | BLogOp And be1 be2 => eval_bexpr f be1 && eval_bexpr f be2
+  | BLogOp Or  be1 be2 => eval_bexpr f be1 || eval_bexpr f be2
+  | BNot be => ~~ eval_bexpr f be
   end
 
-with eval_zexpr ze : int :=
+with eval_zexpr f ze : int :=
   match ze with
   | ZVar v => f v
   | ZConst n => n
-  | ZTest be ze1 ze2 => if eval_bexpr be then eval_zexpr ze1
-                        else eval_zexpr ze2
-  | ZArith Plus ze1 ze2 => eval_zexpr ze1 + eval_zexpr ze2
-  | ZArith Times ze1 ze2 => eval_zexpr ze1 * eval_zexpr ze2
-  | ZArith Minus ze1 ze2 => eval_zexpr ze1 - eval_zexpr ze2
+  | ZTest be ze1 ze2 => if eval_bexpr f be then eval_zexpr f ze1
+                        else eval_zexpr f ze2
+  | ZArith Plus ze1 ze2 => eval_zexpr f ze1 + eval_zexpr f ze2
+  | ZArith Times ze1 ze2 => eval_zexpr f ze1 * eval_zexpr f ze2
+  | ZArith Minus ze1 ze2 => eval_zexpr f ze1 - eval_zexpr f ze2
   | ZTrunc _ _ => 0 (* FIXME *)
   end
 
-with eval_qexpr qe : rat :=
+with eval_qexpr f qe : rat :=
   match qe with
   | QConst x => x
-  | QTest be qe1 qe2 => if eval_bexpr be then eval_qexpr qe1
-                        else eval_qexpr qe2
-  | QArith Plus qe1 qe2 => eval_qexpr qe1 + eval_qexpr qe2
-  | QArith Times qe1 qe2 => eval_qexpr qe1 * eval_qexpr qe2
-  | QArith Minus qe1 qe2 => eval_qexpr qe1 - eval_qexpr qe2
-  | QOfZ ze => ratz (eval_zexpr ze)
+  | QTest be qe1 qe2 => if eval_bexpr f be then eval_qexpr f qe1
+                        else eval_qexpr f qe2
+  | QArith Plus qe1 qe2 => eval_qexpr f qe1 + eval_qexpr f qe2
+  | QArith Times qe1 qe2 => eval_qexpr f qe1 * eval_qexpr f qe2
+  | QArith Minus qe1 qe2 => eval_qexpr f qe1 - eval_qexpr f qe2
+  | QOfZ ze => ratz (eval_zexpr f ze)
+  end.
+
+Fixpoint subst_bexpr f be : bexpr :=
+  match be with
+  | BConst _ => be
+  | BEqB be1 be2 => BEqB (subst_bexpr f be1) (subst_bexpr f be2)
+  | BEqZ ze1 ze2 => BEqZ (subst_zexpr f ze1) (subst_zexpr f ze2)
+  | BEqQ qe1 qe2 => BEqQ (subst_qexpr f qe1) (subst_qexpr f qe2)
+  | BTest be be1 be2 => BTest (subst_bexpr f be) (subst_bexpr f be1) (subst_bexpr f be2)
+  | BCompZ o ze1 ze2 => BCompZ o (subst_zexpr f ze1) (subst_zexpr f ze2)
+  | BCompQ o qe1 qe2 => BCompQ o (subst_qexpr f qe1) (subst_qexpr f qe2)
+  | BLogOp o be1 be2 => BLogOp o (subst_bexpr f be1) (subst_bexpr f be2)
+  | BNot be => BNot (subst_bexpr f be)
+  end
+
+with subst_zexpr f ze : zexpr :=
+  match ze with
+  | ZVar v => f v
+  | ZConst _ => ze
+  | ZTest be ze1 ze2 => ZTest (subst_bexpr f be) (subst_zexpr f ze1) (subst_zexpr f ze2)
+  | ZArith o ze1 ze2 => ZArith o (subst_zexpr f ze1) (subst_zexpr f ze2)
+  | ZTrunc o qe => ZTrunc o (subst_qexpr f qe)
+  end
+
+with subst_qexpr f qe : qexpr :=
+  match qe with
+  | QConst _ => qe
+  | QTest be qe1 qe2 => QTest (subst_bexpr f be) (subst_qexpr f qe1) (subst_qexpr f qe2)
+  | QArith o qe1 qe2 => QArith o (subst_qexpr f qe1) (subst_qexpr f qe2)
+  | QOfZ ze => QOfZ (subst_zexpr f ze)
   end.
 
 End Eval.
@@ -116,3 +164,77 @@ Axiom zexpr_choiceMixin : Choice.mixin_of zexpr.
 Canonical zexpr_choiceType := Eval hnf in ChoiceType zexpr zexpr_choiceMixin.
 Axiom zexpr_ordMixin : Ord.mixin_of zexpr.
 Canonical zexpr_ordType := Eval hnf in OrdType zexpr zexpr_ordMixin.
+
+Fixpoint bexpr_vars be :=
+  match be with
+  | BConst _         => fset0
+  | BEqB be1 be2     => bexpr_vars be1 :|: bexpr_vars be2
+  | BEqZ ze1 ze2     => zexpr_vars ze1 :|: zexpr_vars ze2
+  | BEqQ qe1 qe2     => qexpr_vars qe1 :|: qexpr_vars qe2
+  | BTest be be1 be2 => bexpr_vars be  :|: bexpr_vars be1 :|: bexpr_vars be2
+  | BCompZ _ ze1 ze2 => zexpr_vars ze1 :|: zexpr_vars ze2
+  | BCompQ _ qe1 qe2 => qexpr_vars qe1 :|: qexpr_vars qe2
+  | BLogOp _ be1 be2 => bexpr_vars be1 :|: bexpr_vars be2
+  | BNot be          => bexpr_vars be
+  end
+
+with zexpr_vars ze :=
+  match ze with
+  | ZVar v           => fset1 v
+  | ZConst _         => fset0
+  | ZTest be ze1 ze2 => bexpr_vars be  :|: zexpr_vars ze1 :|: zexpr_vars ze2
+  | ZArith _ ze1 ze2 => zexpr_vars ze1 :|: zexpr_vars ze2
+  | ZTrunc _ qe      => qexpr_vars qe
+  end
+
+with qexpr_vars qe :=
+  match qe with
+  | QConst _         => fset0
+  | QTest be qe1 qe2 => bexpr_vars be  :|: qexpr_vars qe1 :|: qexpr_vars qe2
+  | QArith _ qe1 qe2 => qexpr_vars qe1 :|: qexpr_vars qe2
+  | QOfZ ze          => zexpr_vars ze
+  end.
+
+Ltac solve_expr_varsP :=
+  move=> *;
+  repeat match goal with
+         | [H : is_true (fsubset (_ :|: _) _) |- _] =>
+           rewrite fsubUset in H
+         | [H : is_true (_ && _) |- _] =>
+           case/andP: H=> ??
+         | [IH : ?P -> _, H : ?P |- _] =>
+           move/(_ H) in IH
+         | [H : ?x = _ |- context[?x]] => rewrite {}H
+         | [x : _ |- _] =>
+           match goal with
+           | [ |- context[match x with _ => _ end]] =>
+             case: x=> * /=
+           end
+         end.
+
+Implicit Types V : {fset var}.
+
+Lemma expr_varsP V f g :
+  {in V, f =1 g} ->
+  (forall be, fsubset (bexpr_vars be) V ->
+              eval_bexpr f be = eval_bexpr g be) /\
+  (forall ze, fsubset (zexpr_vars ze) V ->
+              eval_zexpr f ze = eval_zexpr g ze) /\
+  (forall qe, fsubset (qexpr_vars qe) V ->
+              eval_qexpr f qe = eval_qexpr g qe).
+Proof.
+move=> efg; apply: expr_ind=> //=; try by solve_expr_varsP.
+move=> v; rewrite fsub1set; exact: efg.
+Qed.
+
+Lemma bexpr_varsP V f g :
+  {in V, f =1 g} ->
+  forall ze, fsubset (bexpr_vars ze) V ->
+  eval_bexpr f ze = eval_bexpr g ze.
+Proof. by move=> /expr_varsP [? [? ?]]. Qed.
+
+Lemma zexpr_varsP V f g :
+  {in V, f =1 g} ->
+  forall ze, fsubset (zexpr_vars ze) V ->
+  eval_zexpr f ze = eval_zexpr g ze.
+Proof. by move=> /expr_varsP [? [? ?]]. Qed.
