coq/Imp.v
@@ -17,10 +17,27 @@ Unset Strict Implicit.
 Unset Printing Implicit Defensive.
 
 Local Open Scope fset_scope.
+Local Open Scope prob_scope.
+
+(* MOVE *)
+Section FilterMap.
+
+Variables T : ordType.
+Variables S R : Type.
+
+Definition filter_map (f : T -> S -> option R) (m : {fmap T -> S}) : {fmap T -> R} :=
+  mkfmapfp (fun x => obind (f x) (m x)) (domm m).
+
+Lemma filter_mapE f m x : filter_map f m x = obind (f x) (m x).
+Proof.
+by rewrite /filter_map mkfmapfpE mem_domm; case: (m x).
+Qed.
+End FilterMap.
+(* /MOVE *)
 
 Inductive com :=
 | Skip
-| Assn of {fmap var -> zexpr} & com
+| Assn of {fmap var -> {prob zexpr}} & com
 | If of bexpr & com & com & com
 | Block of {fset var} & com & com.
 
@@ -40,7 +57,7 @@ Definition fun_of_state (st : state) (v : var) : int :=
 
 Coercion fun_of_state : state >-> Funclass.
 
-Implicit Types (c : com) (st : state).
+Implicit Types (c : com) (st : state) (φ : state → var → int).
 
 Lemma eq_state st1 st2 : st1 =1 st2 <-> st1 = st2.
 Proof.
@@ -77,19 +94,148 @@ case: (stval st v)=> //=.
 by case: (assn v).
 Qed.
 
-Fixpoint run c st : {prob state} :=
+Fixpoint run φ c st : {prob state} :=
   match c with
   | Skip =>
     dirac st
   | Assn assn c =>
-    sample (mapim_p (fun _ e => dirac (eval_zexpr st e)) assn)
-      (fun assn' => run c (upd st assn'))
+    let eval _ pe := sample: e <- pe; dirac (eval_zexpr (φ st) e) in
+    sample: assn' <- mapim_p eval assn;
+    run φ c (upd st assn')
   | If e cthen celse c =>
-    let branch := if eval_bexpr st e then cthen else celse in
-    sample (run branch st) (run c)
+    let branch := if eval_bexpr (φ st) e then cthen else celse in
+    sample (run φ branch st) (run φ c)
   | Block vs block c =>
     let old := state_of_fun vs st in
     let new := upd st (mkfmapf (fun _ => 0%R) vs) in
-    sample (run block new)
-      (fun st' => run c (upd st' (mkfmapf old vs)))
+    sample: st' <- run φ block new;
+    run φ c (upd st' (mkfmapf old vs))
   end.
+
+Record renaming := Renaming {
+  ren_val : {fmap var → var};
+  _       : all (fun v => ren_val v != Some v) (domm ren_val);
+}.
+
+Canonical renaming_subType := [subType for ren_val].
+
+Definition fun_of_renaming (r : renaming) v :=
+  if val r v is Some v' then v' else v.
+
+Coercion fun_of_renaming : renaming >-> Funclass.
+
+Module Inlining.
+
+Definition fresh_for (fv : {fmap string → nat}) (V : {fset var}) :=
+  ∀ x n, Var x n \in V → if fv x is Some m then n <= m else false.
+
+Record istate := IState {
+  fresh_vars  : {fmap string → nat};
+  formulas    : seq (var * zexpr);
+  used_vars   : {fmap var → {fset var}};
+  ren         : renaming;
+}.
+
+Definition M T : Type := istate → istate * T.
+
+Definition ret T (x : T) : M T :=
+  fun s => (s, x).
+
+Definition bind T S (x : M T) (f : T → M S) : M S :=
+  fun s => f (x s).2 (x s).1.
+
+Notation "'bind:' x '<-' t1 ';' t2" :=
+  (bind t1 (fun x => t2))
+  (at level 20, t1 at level 100, t2 at level 200,
+   right associativity, format "'[' 'bind:'  x  '<-'  '[' t1 ;  ']' ']' '/' t2 ").
+
+Definition get T (f : istate → T) : M T :=
+  fun s => (s, f s).
+
+Definition mod (f : istate → istate) : M unit :=
+  fun s => (f s, tt).
+
+Definition set_fresh_vars fv : M unit :=
+  mod (fun '(IState _ f u r) => IState fv f u r).
+
+Definition fresh (x : string) : M var :=
+  bind: fv <- get fresh_vars;
+  if fv x is Some m then
+    bind: _ <- set_fresh_vars (setm fv x m.+1);
+    ret (Var x m)
+  else
+    bind: _ <- set_fresh_vars (setm fv x 0);
+    ret (Var x 0).
+
+Definition intern_var (v : var) (e : zexpr) : M unit :=
+  bind: v' <- fresh (vname v);
+  bind: u  <- get used_vars;
+  let vs := \bigcup_(v'' <- zexpr_vars e) u v'' in
+  mod (fun '(IState fv fs uv r) => IState fv ((v', e) :: fs)
+
+Fixpoint inline_loop (c : com) : M com :=
+  match c with
+  | Skip =>
+    ret Skip
+  | Assn assn c =>
+    let det_assn := filter_map (fun=> of_dirac) assn in
+    if domm det_assn == domm assn then
+      bind: r <- get renaming;
+      let det_assn := mapm (subst_zexpr (ZVar \o r)) det_assn in
+
+
+
+Definition spec T (P : istate → Prop) (x : M T) (Q : T → istate → Prop) : Prop :=
+  ∀ s, P s → Q (x s).2 (x s).1.
+
+
+
+
+
+
+
+
+
+Fixpoint com_read_vars c : {fset var} :=
+  match c with
+  | Skip =>
+    fset0
+  | Assn assn c =>
+    com_read_vars c :|:
+    \bigcup_(pe <- codomm assn)
+    \bigcup_(e  <- supp pe) zexpr_vars e
+  | If be cthen celse c =>
+    bexpr_vars be :|:
+    com_read_vars cthen :|:
+    com_read_vars celse :|:
+    com_read_vars c
+  | Block vs block c =>
+    (com_read_vars block :\: vs) :|:
+    com_read_vars c
+  end.
+
+Lemma com_read_varsP (V : {fset var}) c st1 st2 :
+  {in V, st1 =1 st2} ->
+  fsubset (com_read_vars c) V ->
+  forall st1', st1' \in supp (run c st1) ->
+  forall st2', st2' \in supp (run c st2) ->
+  {in V, st1' =1 st2'}.
+Proof.
+elim: c st1 st2=> //=.
+- by move=> ??? _ _ /supp_diracP -> _ /supp_diracP ->.
+- move=> assn c IH st1 st2 e.
+  rewrite fsubUset; case/andP=> sub_c sub_assn.
+  move=> st1' /supp_sampleP [/= vals1 vals1P st1'P].
+  move=> st2' /supp_sampleP [/= vals2 vals2P st2'P].
+  have {}e: {in V, upd st1 vals1 =1 upd st2 vals2}.
+    admit.
+  by apply: IH; eauto.
+- move=> be cthen IHthen celse IHelse c IH st1 st2 e.
+  rewrite !fsubUset -!andbA; case/and4P=> sub_be sub_cthen sub_celse sub_c.
+  move=> st1'' /supp_sampleP [/= st1' st1'P st1''P].
+  move=> st2'' /supp_sampleP [/= st2' st2'P st2''P].
+  rewrite -(bexpr_varsP e sub_be) in st2'P.
+  suff ?: {in V, st1' =1 st2'} by eauto using IH.
+  case: eval_bexpr in st1'P st2'P.
+  + by eauto using IHthen.
+  + by eauto using IHelse.
